did some more testing with VCV & implementing prover execution

Tutorials/TestVCV.lean
@@ -1,1 +1,86 @@
 import VCVio
+
+open Sum Polynomial OracleSpec OracleComp
+
+variable {α β γ : Type} [Inhabited β] [Fintype β]
+    [DecidableEq β] [DecidableEq α] [Inhabited γ] [Fintype γ]
+
+-- Given a computation that answers queries, construct a `SimOracle`
+def statelessOracle {ι ι' : Type} {spec : OracleSpec ι} {spec' : OracleSpec ι'}
+    (f : (i : ι) → spec.domain i → OracleComp spec' (spec.range i)) :
+    spec →[Unit]ₛₒ spec' :=
+  λ i t () ↦ (·, ()) <$> f i t
+
+-- turn a function into an oracle implementation, while logging queries
+-- the stateless oracle introduces a useless `Unit` to the internal state which we mask
+-- `simulate` with this will answer queries with `f` and log input and outputs
+def oracleize (f : α → β) : (α →ₒ β) →[QueryLog (α →ₒ β)]ₛₒ (α →ₒ β) :=
+  (loggingOracle ∘ₛₒ statelessOracle (λ () t ↦ return f t)).maskState
+    (Equiv.punitProd (α →ₒ β).QueryLog)
+
+
+
+-- Lifting a deterministic function `f: α → β` to an oracle that keeps track of the queries
+-- def oracleize (f : α → β) : SimOracle (α →ₒ β) (α →ₒ β) (QueryLog (α →ₒ β)) :=
+--   fun _ a log => do
+--     let b := f a
+--     return (b, QueryLog.logQuery log a b)
+
+-- Testing the oracle-ize operation
+def testOracleize (f : α → β) (a : α) : OracleComp (α →ₒ β) (β × (α →ₒ β).QueryLog) := do
+  let (y, s) ← simulate (oracleize f) (fun _ => []) (pure (f a))
+  let (z, s') ← simulate (oracleize f) s (pure y)
+  return (z, s')
+
+#check testOracleize (fun (x : Bool) => Not x) true
+
+-- #eval OracleComp.runIO (runDeterministic (fun (x : Bool) => not x) true)
+-- Since the computation is deterministic, can I return the actual value?
+
+
+-- Well... since all I really need is to add a wrapper to a function, that additionally keeps track of the queries, I could just define my own thing
+-- inductive OracleWithLog {α β : Type} (log : List (α × β)) : Type where
+--   | init : OracleWithLog (List.nil)
+--   | query : (a : α) → OracleWithLog log → OracleWithLog (log ++ [(a, f a)])
+--   | return : β → OracleWithLog log
+
+
+variable {R : Type} [Semiring R]
+  [Fintype R] [DecidableEq R] [Inhabited R]
+  [SelectableType R]
+
+-- Second oracle take in values in `R` and "evaluate" the polynomial on them
+-- At this point oracle is a black box, no actual behavior specified
+-- But for the purpose of defining the computation that isn't needed
+def test : OracleComp (unifSpec ++ₒ (R →ₒ R)) R := do
+  let x₁ : R ←$ᵗ R
+  let x₂ : R ←$ᵗ R
+  -- Query the `inr` oracle to evaluate polynomial on some values
+  let query_result₁ : R ← query (inr ()) (x₁ + x₂)
+  let query_result₂ : R ← query (inr ()) (x₁ + 2 * x₂)
+  return query_result₁ + query_result₂
+
+-- `SimOracle` for actually implementing oracle behavior
+-- Simulates the oracle `R →ₒ R` by evaluating the polynomial on queries
+-- This reduces the oracles to just `unifSpec` (although really anything could go there)
+-- Assumes the polynomial is globally fixed so just take `p` as input
+-- No internal state so we use `Unit` type for that
+def polyEvalOracle (p : R[X]) : (R →ₒ R) →[Unit]ₛₒ emptySpec :=
+  λ () t () ↦ do
+    let eval_result := p.eval t
+    return (eval_result, ())
+
+-- Run a computation `oa : OracleComp (unifSpec ++ₒ (R →ₒ R)) α` using the above
+-- `polyGenerator` is the computation that produces the polynomial to use for oracle
+noncomputable example (p : R[X])
+    (oa : OracleComp (R →ₒ R) α) :
+    OracleComp emptySpec α := do
+  let x ← simulate' (idOracle ++ₛₒ polyEvalOracle p) ((), ()) oa
+  return x
+
+-- Version that stores the polynomial in state of the oracle
+-- Only needed if the polynomial being used will change during the execution
+def polyEvalOracle_state : (R →ₒ R) →[R[X]]ₛₒ unifSpec :=
+  λ () t p ↦ do
+    let eval_result := p.eval t
+    return (eval_result, p) -- Could modify the internal polynomial `p` first
