Tutorials/Execution.lean
@@ -1,0 +1,51 @@
+import Mathlib.Data.Fin.Basic
+import Mathlib.Data.PNat.Basic
+
+structure EvolvingProver where
+  n : PNat
+  State : Fin (n + 1) → Type
+  Input : Fin n → Type
+  Output : Fin n → Type
+  step : (i : Fin n) → Input i → State i → (Output i × State i.succ)
+
+theorem test {n : ℕ+} (i : Fin (n + 1)) (h : i = 0) : Fin.val i = 0 := by
+  exact Fin.eq_mk_iff_val_eq.mp h
+
+def runEvolvingProverAux {ep : EvolvingProver}
+  (i : Fin (ep.n + 1))
+  (inputs : (j : Fin i) → ep.Input j)
+  (initialState : ep.State 0) :
+  ((j : Fin i) → ep.Output j) × ep.State i :=
+    if h : i = 0 then
+      (λ j => False.elim (Fin.elim0 (Fin.cast (Fin.eq_mk_iff_val_eq.mp h) j)), h ▸ initialState)
+    else
+        let i' : Fin ep.n := Fin.pred i h
+        let ⟨prevOut, prevState⟩ := runEvolvingProverAux i' (λ j => inputs (Fin.castLT j)) initialState
+        let (output, nextState) := ep.step i' (inputs i') prevState
+        (λ j =>
+          if h' : j.val < i'.val then
+            prev.1 (Fin.castLT j)
+          else
+            cast (by rw [show j = i' from Fin.eq_of_val_eq (Nat.le_antisymm (Nat.le_of_lt_succ (Fin.is_lt j)) (Nat.le_of_not_lt h'))]) output,
+        nextState)
+
+-- Example usage:
+def exampleProver : EvolvingProver := {
+  n := 3
+  State := λ i => match i with
+    | 0 => Nat
+    | 1 => String
+    | 2 => Bool
+    | 3 => Unit
+    | _ => Unit  -- This case is unreachable but needed for exhaustiveness
+  Input := λ _ => Nat
+  Output := λ _ => String
+  step := λ i input state =>
+    match i, state with
+    | 0, s => ("Output 0", "State 1")
+    | 1, s => ("Output 1", true)
+    | 2, s => ("Output 2", ())
+    | _ => ("", ())  -- This case is unreachable but needed for exhaustiveness
+}
+
+#eval runEvolvingProverAllRounds (λ _ => 0) 0
